Fix soundness theorem for modal logic

Logic/Modal/Normal/Logics.lean
@@ -18,17 +18,18 @@ variable {F : Type u} [ModalLogicSymbol F] {p q : F}
 abbrev Logic (F : Type u) [ModalLogicSymbol F] := Set F
 
 
-abbrev LogicK : Logic F := AxiomK.ctx
+abbrev LogicK : Logic F := 𝐊
+notation "𝐊" => LogicK.ctx
 
 namespace LogicK
 
 @[simp] lemma includes_AxiomK : (AxiomK p q) ∈ 𝐊 := by simp [LogicK]
-@[simp] lemma subsets_AxiomK : AxiomK.ctx ⊆ (𝐊 : Logic F) := by simp [LogicK];
+@[simp] lemma subsets_AxiomK : 𝐊 ⊆ (𝐊 : Logic F) := by simp [LogicK];
 
 end LogicK
 
 
-def LogicKD : Logic F := 𝐊 ∪ AxiomD.ctx
+def LogicKD : Logic F := 𝐊 ∪ 𝐃
 notation "𝐊𝐃" => LogicKD
 
 /-
@@ -51,7 +52,7 @@ abbrev LogicK45 : Logic F := AxiomK ∪ 𝟒 ∪ 𝟓
 abbrev LogicK5 : Logic F := AxiomK ∪ 𝟓
 -/
 
-def LogicKT4 : Logic F := 𝐊 ∪ AxiomT.ctx ∪ Axiom4.ctx
+def LogicKT4 : Logic F := 𝐊 ∪ 𝐓 ∪ 𝟒
 
 @[simp] abbrev LogicS4 {F} := @LogicKT4 F
 notation "𝐒𝟒" => LogicS4
@@ -61,14 +62,14 @@ namespace LogicS4
 @[simp] lemma includes_AxiomK : AxiomK p q ∈ (𝐒𝟒 : Logic F) := by simp [LogicKT4]
 @[simp] lemma includes_AxiomT : AxiomT p ∈ (𝐒𝟒 : Logic F) := by simp [LogicKT4]
 @[simp] lemma includes_Axiom4 : Axiom4 p ∈ (𝐒𝟒 : Logic F) := by simp [LogicKT4]
-@[simp] lemma subsets_K : AxiomK.ctx ⊆ (𝐒𝟒 : Logic F) := by apply Set.subset_triunion₁
-@[simp] lemma subsets_T : AxiomT.ctx ⊆ (𝐒𝟒 : Logic F) := by apply Set.subset_triunion₂
-@[simp] lemma subsets_4 : Axiom4.ctx ⊆ (𝐒𝟒 : Logic F) := by apply Set.subset_triunion₃
+@[simp] lemma subsets_K : 𝐊 ⊆ (𝐒𝟒 : Logic F) := by apply Set.subset_triunion₁
+@[simp] lemma subsets_T : 𝐓 ⊆ (𝐒𝟒 : Logic F) := by apply Set.subset_triunion₂
+@[simp] lemma subsets_4 : 𝟒 ⊆ (𝐒𝟒 : Logic F) := by apply Set.subset_triunion₃
 
 end LogicS4
 
 
-def LogicS4Dot2 : Logic F := 𝐒𝟒 ∪ AxiomDot2.ctx
+def LogicS4Dot2 : Logic F := 𝐒𝟒 ∪ .𝟐
 
 notation "𝐒𝟒.𝟐" => LogicS4Dot2
 
@@ -81,7 +82,7 @@ namespace LogicS4Dot2
 end LogicS4Dot2
 
 
-def LogicS4Dot3 : Logic F := 𝐒𝟒 ∪ AxiomDot3.ctx
+def LogicS4Dot3 : Logic F := 𝐒𝟒 ∪ .𝟑
 notation "𝐒𝟒.𝟑" => LogicS4Dot3
 
 namespace LogicS4Dot3
@@ -93,7 +94,7 @@ namespace LogicS4Dot3
 end LogicS4Dot3
 
 
-def LogicS4Grz : Logic F := 𝐒𝟒 ∪ AxiomGrz.ctx
+def LogicS4Grz : Logic F := 𝐒𝟒 ∪ 𝐆𝐫𝐳
 notation "𝐒𝟒𝐆𝐫𝐳" => LogicS4Grz
 
 namespace LogicS4Grz
@@ -105,7 +106,7 @@ namespace LogicS4Grz
 end LogicS4Grz
 
 
-def LogicKT5 : Logic F := 𝐊 ∪ AxiomT.ctx ∪ 𝟓
+def LogicKT5 : Logic F := 𝐊 ∪ 𝐓 ∪ 𝟓
 
 @[simp] abbrev LogicS5 {F} := @LogicKT5 F
 notation "𝐒𝟓" => LogicS5
@@ -115,22 +116,22 @@ namespace LogicS5
 @[simp] lemma includes_AxiomK : AxiomK p q ∈ (𝐒𝟓 : Logic F) := by simp [LogicKT5]
 @[simp] lemma includes_AxiomT : AxiomT p ∈ (𝐒𝟓 : Logic F) := by simp [LogicKT5]
 @[simp] lemma includes_Axiom5 : Axiom5 p ∈ (𝐒𝟓 : Logic F) := by simp [LogicKT5]
-@[simp] lemma subsets_K : AxiomK.ctx ⊆ (𝐒𝟓 : Logic F) := by apply Set.subset_triunion₁
-@[simp] lemma subsets_T : AxiomT.ctx ⊆ (𝐒𝟓 : Logic F) := by apply Set.subset_triunion₂
-@[simp] lemma subsets_5 : Axiom5.ctx ⊆ (𝐒𝟓 : Logic F) := by apply Set.subset_triunion₃
+@[simp] lemma subsets_K : 𝐊 ⊆ (𝐒𝟓 : Logic F) := by apply Set.subset_triunion₁
+@[simp] lemma subsets_T : 𝐓 ⊆ (𝐒𝟓 : Logic F) := by apply Set.subset_triunion₂
+@[simp] lemma subsets_5 : 𝟓 ⊆ (𝐒𝟓 : Logic F) := by apply Set.subset_triunion₃
 
 end LogicS5
 
 
-def LogicGL : Logic F := 𝐊 ∪ AxiomL.ctx
+def LogicGL : Logic F := 𝐊 ∪ 𝐋
 notation "𝐆𝐋" => LogicGL
 
 namespace LogicGL
 
 @[simp] lemma includes_AxiomK : AxiomK p q ∈ (𝐆𝐋 : Logic F) := by simp [LogicGL]
 @[simp] lemma includes_AxiomL : AxiomL p ∈ (𝐆𝐋 : Logic F) := by simp [LogicGL]
-@[simp] lemma subsets_K : AxiomK.ctx ⊆ (𝐆𝐋 : Logic F) := by simp [LogicGL, LogicK]
-@[simp] lemma subsets_L : AxiomL.ctx ⊆ (𝐆𝐋 : Logic F) := by simp [LogicGL]
+@[simp] lemma subsets_K : 𝐊 ⊆ (𝐆𝐋 : Logic F) := by simp [LogicGL, LogicK]
+@[simp] lemma subsets_L : 𝐋 ⊆ (𝐆𝐋 : Logic F) := by simp [LogicGL]
 @[simp] lemma subsets_LogicK_ctx : 𝐊 ⊆ (𝐆𝐋 : Logic F) := by simp [LogicK, LogicGL]
 
 end LogicGL
